Gates.v
@@ -11,6 +11,8 @@ Definition ZX_H :=
             (Z_Spider 1 1 (PI/2)))).
 Global Opaque ZX_H.
 
+Notation nH := (nStack1 ZX_H).
+
 Definition ZX_CNOT_l : ZX 2 2 := 
     (Compose 
         (Stack 
